- 6.1.1 \
 c0 = $lambda . lambda . 0$ \
 c2 = $lambda . lambda . 1 space (1 space 0)$ \
 plus = $lambda . lambda . lambda . lambda . 3 space 1 space (2 space 0 space 1)$ \
 fix = $lambda . (lambda . 1 space (lambda . (1 space 1) space 0)) (lambda . 1 (lambda . (1 space 1) 0))$ \
 foo = $(lambda . (lambda . 0)) (lambda . 0)$ \
 
- 6.2.2 \
  1. $(lambda . lambda . 1 (0 space 4))$ \ 
  2. $(lambda . 0 space 1 space (lambda . 0 space 1 space 4))$

- 6.2.5 \
  1. $[0 arrow 1] (0 (lambda . lambda . 2))$
  2. $[0 arrow 1 (lambda . 2)] (0 (lambda . 1))$
  3. $[0 arrow 1] (lambda . 0 space 2)$
  4. $[0 arrow 1] (lambda . 1 space 0)$
